Port optimization metatheory

src/model/Global.v
@@ -115,4 +115,53 @@ Module Global.
     apply Memory.cap_messages_le.
     apply Memory.cap_of_cap.
   Qed.
+
+  Variant strong_le (gl1 gl2: t): Prop :=
+  | strong_le_intro
+      (LE: le gl1 gl2)
+      (ADDNA: forall loc,
+          (<<PROMISES: implb (gl1.(promises) loc) (gl2.(promises) loc)>>) \/
+          (<<LATEST: Memory.na_added_latest loc gl1.(memory) gl2.(memory)>>))
+  .
+  #[global] Hint Constructors strong_le: core.
+
+  Global Program Instance strong_le_PreOrder: PreOrder strong_le.
+  Next Obligation.
+    ii. destruct x. econs; [refl|]. i. left. ss. rewrite Bool.implb_same. auto.
+  Qed.
+  Next Obligation.
+    ii. destruct x, y, z. inv H. inv H0. ss. econs.
+    { etrans; eauto. }
+    { i. ss. destruct (promises0 loc) eqn:PRM0.
+      { destruct (promises2 loc) eqn:PRM2.
+        { left. ss. }
+        destruct (promises1 loc) eqn:PRM1.
+        { right. hexploit ADDNA0; eauto.
+          rewrite PRM1. rewrite PRM2. i. des; ss.
+          eapply Memory.na_added_latest_le.
+          { inv LE. eauto. }
+          { eauto. }
+          { reflexivity. }
+        }
+        { right. hexploit ADDNA; eauto.
+          rewrite PRM0. rewrite PRM1. i. des; ss.
+          eapply Memory.na_added_latest_le.
+          { reflexivity. }
+          { eauto. }
+          { inv LE0. eauto. }
+        }
+      }
+      econs; etrans; eauto.
+    }
+  Qed.
+
+  Lemma cap_strong_le
+    gl gl_cap
+    (CAP: gl_cap = cap_of gl):
+    strong_le gl gl_cap.
+  Proof.
+    destruct gl, gl_cap. inv CAP. econs.
+    { eapply cap_le; eauto. }
+    { i. left. ss. rewrite Bool.implb_same. auto. }
+  Qed.
 End Global.
