src/trans/SimMemory.v
@@ -185,6 +185,401 @@ Proof.
     + inv H. inv MSG. ss.
 Qed.
 
+Lemma sim_memory_add_exist
+      mem1_src mem1_tgt msg_src
+      mem2_tgt msg_tgt
+      loc from to
+      (MSG: Message.le msg_src msg_tgt)
+      (MWF: Message.wf msg_src)
+      (TGT: Memory.add mem1_tgt loc from to msg_tgt mem2_tgt)
+      (SIM: sim_memory mem1_src mem1_tgt):
+  exists mem2_src,
+    (<<ADD: Memory.add mem1_src loc from to msg_src mem2_src>>) /\
+      (<<SIM: sim_memory mem2_src mem2_tgt>>).
+Proof.
+  assert (exists mem2_src, <<SRC: Memory.add mem1_src loc from to msg_src mem2_src>>).
+  { apply Memory.add_exists.
+    { eapply covered_disjoint.
+      { inv SIM. eapply COVER. }
+      { inv TGT. inv ADD. eauto. }
+    }
+    { inv TGT. inv ADD. eauto. }
+    { eauto. }
+  }
+  des. hexploit sim_memory_add; eauto.
+Qed.
+
+Lemma sim_memory_remove
+      mem1_src mem1_tgt
+      mem2_src mem2_tgt
+      loc from to
+      (SRC: Memory.remove mem1_src loc from to Message.reserve mem2_src)
+      (TGT: Memory.remove mem1_tgt loc from to Message.reserve mem2_tgt)
+      (SIM: sim_memory mem1_src mem1_tgt):
+  sim_memory mem2_src mem2_tgt.
+Proof.
+  inv SIM. econs; i.
+  - rewrite remove_covered; [|eauto]. rewrite (@remove_covered mem2_tgt); [|eauto].
+    econs; i; des; (try by right).
+    { splits; auto. eapply COVER; eauto. }
+    { splits; auto. eapply COVER; eauto. }
+    { splits; auto. eapply COVER; eauto. }
+    { splits; auto. eapply COVER; eauto. }
+  - hexploit MSG; eauto.
+    { erewrite Memory.remove_o in GET; eauto. des_ifs; eauto. }
+    i. des. esplits; eauto.
+    erewrite Memory.remove_o in GET; eauto.
+    erewrite Memory.remove_o; eauto. des_ifs. eauto.
+  - erewrite (@Memory.remove_o mem2_src); try exact SRC.
+    erewrite (@Memory.remove_o mem2_tgt); try exact TGT.
+    condtac; ss.
+Qed.
+
+Lemma sim_memory_adjacent_src
+      mem_src mem_tgt
+      loc from1 to1 from2 to2
+      (SIM: sim_memory mem_src mem_tgt)
+      (CLOSED_SRC: Memory.closed mem_src)
+      (CLOSED_TGT: Memory.closed mem_tgt)
+      (ADJ: Memory.adjacent loc from1 to1 from2 to2 mem_src)
+      (TS: Time.lt to1 from2):
+  exists from1' to2',
+    Memory.adjacent loc from1' to1 from2 to2' mem_tgt.
+Proof.
+  dup SIM. inv SIM0. inv ADJ. clear TS0.
+  assert (GET1_TGT: exists from1' m1', Memory.get loc to1 mem_tgt = Some (from1', m1')).
+  { exploit Memory.get_ts; try exact GET1. i. des.
+    { subst. esplits. eapply CLOSED_TGT. }
+    destruct (COVER loc to1). exploit H.
+    { econs; try exact GET1. econs; eauto. refl. }
+    intros x. inv x. inv ITV. ss. inv TO; cycle 1.
+    { inv H1. esplits; eauto. }
+    exfalso.
+    destruct (Time.le_lt_dec to from2).
+    { exploit MSG; eauto. i. des.
+      exploit (EMPTY to); eauto. i. congr. }
+    destruct (COVER loc from2). exploit H3.
+    { econs; eauto. econs; ss.
+      - etrans; eauto.
+      - econs; ss.
+    }
+    intros x. inv x. inv ITV. ss. inv TO.
+    - exploit Memory.get_ts; try exact GET2. i. des.
+      { subst. inv FROM0. }
+      exploit Memory.get_ts; try exact GET0. i. des.
+      { subst. inv H4. }
+      exploit Memory.get_disjoint; [exact GET2|exact GET0|..]. i. des.
+      { timetac. }
+      destruct (Time.le_lt_dec to2 to0).
+      + apply (x3 to2); econs; ss; try refl.
+        etrans; try exact FROM0. ss.
+      + apply (x3 to0); econs; ss; try refl.
+        econs. ss.
+    - inv H4. exploit (EMPTY to0); eauto; try refl. i. congr.
+  }
+  assert (GET2_TGT: exists to2' m2', Memory.get loc to2' mem_tgt = Some (from2, m2')).
+  { exploit Memory.get_ts; try exact GET2. i. des.
+    { subst. inv TS. }
+    exploit Memory.max_ts_spec; try exact GET2. i. des.
+    clear from msg GET.
+    erewrite sim_memory_max_ts in MAX; eauto.
+    exploit TimeFacts.lt_le_lt; try exact x0; try exact MAX. i.
+    exploit Memory.next_exists; try exact x1; try eapply CLOSED_TGT. i. des.
+    destruct (TimeFacts.le_lt_dec from from2).
+    - inv l; cycle 1.
+      { inv H. esplits; eauto. }
+      destruct (COVER loc from2). exploit H1.
+      { econs; try exact x2. econs; ss. econs; ss. }
+      intros x. inv x. inv ITV. ss. inv TO; cycle 1.
+      { inv H2. exploit (EMPTY to0); eauto; try refl. i. congr. }
+      exploit Memory.get_disjoint; [exact GET2|exact GET|..]. i. des.
+      { subst. timetac. }
+      exfalso.
+      destruct (TimeFacts.le_lt_dec to2 to0).
+      + apply (x5 to2); econs; ss; try refl.
+        etrans; try exact FROM. ss.
+      + apply (x5 to0); econs; ss; try refl.
+        * econs. ss.
+        * etrans; eauto.
+    - destruct (TimeFacts.le_lt_dec to2 from).
+      + destruct (COVER loc to2). exploit H.
+        { econs; eauto. econs; ss. refl. }
+        intros x. inv x. inv ITV. ss.
+        exploit (x4 to0); eauto; try congr.
+        { eapply TimeFacts.lt_le_lt; try exact TO; ss. }
+        destruct (Time.le_lt_dec to to0); ss.
+        exploit Memory.get_ts; try exact x2. i. des.
+        { subst. inv x3. }
+        exploit Memory.get_disjoint; [exact x2|exact GET|..]. i. des.
+        { subst. timetac. }
+        exfalso.
+        apply (x6 to); econs; ss; try refl.
+        etrans; try exact FROM.
+        eapply TimeFacts.le_lt_lt; try exact x5. ss.
+      + destruct (COVER loc from). exploit H.
+        { econs; try exact GET2. econs; ss. econs. ss. }
+        intros x. inv x. inv ITV. ss.
+        destruct (TimeFacts.le_lt_dec to to0).
+        * exploit Memory.get_ts; try exact x2. i. des.
+          { subst. inv x3. }
+          exploit Memory.get_ts; try exact GET. i. des.
+          { subst. timetac. }
+          exploit Memory.get_disjoint; [exact x2|exact GET|..]. i. des.
+          { subst. timetac. }
+          exfalso.
+          apply (x7 to); econs; ss; try refl.
+          eapply TimeFacts.lt_le_lt; try exact FROM. econs. ss.
+        * exploit (x4 to0); ss; try congr.
+          eapply TimeFacts.lt_le_lt; try exact TO; ss.
+  }
+  des. esplits. econs; eauto; i.
+  { exploit Memory.get_ts; try exact GET2_TGT. i. des.
+    - subst. inv TS.
+    - etrans; eauto. }
+  destruct (Memory.get loc ts mem_tgt) as [[]|] eqn:GET; ss.
+  exfalso.
+  exploit Memory.get_ts; try exact GET. i. des.
+  { subst. inv TS1. }
+  destruct (COVER loc ts). exploit H0.
+  { econs; eauto. econs; ss. refl. }
+  intros x. inv x. inv ITV. ss.
+  destruct (TimeFacts.le_lt_dec to from2).
+  { exploit (EMPTY to); try congr.
+    eapply TimeFacts.lt_le_lt; try exact TS1. ss. }
+  exploit Memory.get_ts; try exact GET2. i. des.
+  { subst. inv TS. }
+  exploit Memory.get_ts; try exact GET0. i. des.
+  { subst. inv l. }
+  exploit Memory.get_disjoint; [exact GET2|exact GET0|..]. i. des.
+  { subst. timetac. }
+  destruct (TimeFacts.le_lt_dec to2 to).
+  - apply (x3 to2); econs; ss; try refl.
+    etrans; try exact x1.
+    eapply TimeFacts.lt_le_lt; try exact TS2. ss.
+  - apply (x3 to); econs; ss; try refl. econs. ss.
+Qed.
+
+Lemma sim_memory_adjacent_tgt
+      mem_src mem_tgt
+      loc from1 to1 from2 to2
+      (SIM: sim_memory mem_src mem_tgt)
+      (CLOSED_SRC: Memory.closed mem_src)
+      (CLOSED_TGT: Memory.closed mem_tgt)
+      (ADJ: Memory.adjacent loc from1 to1 from2 to2 mem_tgt)
+      (TS: Time.lt to1 from2):
+  exists from1' to2',
+    Memory.adjacent loc from1' to1 from2 to2' mem_src.
+Proof.
+  dup SIM. inv SIM0. inv ADJ. clear TS0.
+  assert (GET1_SRC: exists from1' m1', Memory.get loc to1 mem_src = Some (from1', m1')).
+  { exploit MSG; try exact GET1. i. des. eauto. }
+  assert (GET2_SRC: exists to2' m2', Memory.get loc to2' mem_src = Some (from2, m2')).
+  { exploit Memory.get_ts; try exact GET2. i. des.
+    { subst. inv TS. }
+    exploit Memory.max_ts_spec; try exact GET2. i. des.
+    clear from msg GET.
+    erewrite <- sim_memory_max_ts in MAX; eauto.
+    exploit TimeFacts.lt_le_lt; try exact x0; try exact MAX. i.
+    exploit Memory.next_exists; try exact x1; try eapply CLOSED_SRC. i. des.
+    destruct (TimeFacts.le_lt_dec from from2).
+    - inv l; cycle 1.
+      { inv H. esplits; eauto. }
+      destruct (COVER loc from2). exploit H0.
+      { econs; try exact x2. econs; ss. econs; ss. }
+      intros x. inv x. inv ITV. ss. inv TO; cycle 1.
+      { inv H2. exploit (EMPTY to0); eauto; try refl. i. congr. }
+      exploit Memory.get_disjoint; [exact GET2|exact GET|..]. i. des.
+      { subst. timetac. }
+      exfalso.
+      destruct (TimeFacts.le_lt_dec to2 to0).
+      + apply (x5 to2); econs; ss; try refl.
+        etrans; try exact FROM. ss.
+      + apply (x5 to0); econs; ss; try refl.
+        * econs. ss.
+        * etrans; eauto.
+    - destruct (TimeFacts.le_lt_dec to2 from).
+      + destruct (COVER loc to2). exploit H0.
+        { econs; eauto. econs; ss. refl. }
+        intros x. inv x. inv ITV. ss.
+        exploit (x4 to0); eauto; try congr.
+        { eapply TimeFacts.lt_le_lt; try exact TO; ss. }
+        destruct (Time.le_lt_dec to to0); ss.
+        exploit Memory.get_ts; try exact x2. i. des.
+        { subst. inv x3. }
+        exploit Memory.get_disjoint; [exact x2|exact GET|..]. i. des.
+        { subst. timetac. }
+        exfalso.
+        apply (x6 to); econs; ss; try refl.
+        etrans; try exact FROM.
+        eapply TimeFacts.le_lt_lt; try exact x5. ss.
+      + destruct (COVER loc from). exploit H0.
+        { econs; try exact GET2. econs; ss. econs. ss. }
+        intros x. inv x. inv ITV. ss.
+        destruct (TimeFacts.le_lt_dec to to0).
+        * exploit Memory.get_ts; try exact x2. i. des.
+          { subst. inv x3. }
+          exploit Memory.get_ts; try exact GET. i. des.
+          { subst. timetac. }
+          exploit Memory.get_disjoint; [exact x2|exact GET|..]. i. des.
+          { subst. timetac. }
+          exfalso.
+          apply (x7 to); econs; ss; try refl.
+          eapply TimeFacts.lt_le_lt; try exact FROM. econs. ss.
+        * exploit (x4 to0); ss; try congr.
+          eapply TimeFacts.lt_le_lt; try exact TO; ss.
+  }
+  des. esplits. econs; eauto; i.
+  { exploit Memory.get_ts; try exact GET2_SRC. i. des.
+    - subst. inv TS.
+    - etrans; eauto. }
+  destruct (Memory.get loc ts mem_src) as [[]|] eqn:GET; ss.
+  exfalso.
+  exploit Memory.get_ts; try exact GET. i. des.
+  { subst. inv TS1. }
+  destruct (COVER loc ts). exploit H.
+  { econs; eauto. econs; ss. refl. }
+  intros x. inv x. inv ITV. ss.
+  destruct (TimeFacts.le_lt_dec to from2).
+  { exploit (EMPTY to); try congr.
+    eapply TimeFacts.lt_le_lt; try exact TS1. ss. }
+  exploit Memory.get_ts; try exact GET2. i. des.
+  { subst. inv TS. }
+  exploit Memory.get_ts; try exact GET0. i. des.
+  { subst. inv l. }
+  exploit Memory.get_disjoint; [exact GET2|exact GET0|..]. i. des.
+  { subst. timetac. }
+  destruct (TimeFacts.le_lt_dec to2 to).
+  - apply (x3 to2); econs; ss; try refl.
+    etrans; try exact x1.
+    eapply TimeFacts.lt_le_lt; try exact TS2. ss.
+  - apply (x3 to); econs; ss; try refl. econs. ss.
+Qed.
+
+Lemma sim_memory_cap_get_src
+      mem1_src mem2_src
+      mem1_tgt mem2_tgt
+      loc from to msg
+      (MEM1: sim_memory mem1_src mem1_tgt)
+      (CAP_SRC: Memory.cap mem1_src mem2_src)
+      (CAP_TGT: Memory.cap mem1_tgt mem2_tgt)
+      (MEM1_SRC: Memory.closed mem1_src)
+      (MEM1_TGT: Memory.closed mem1_tgt)
+      (GET1_SRC: Memory.get loc to mem1_src = None)
+      (GET2_SRC: Memory.get loc to mem2_src = Some (from, msg)):
+  <<MSG: msg = Message.reserve>> /\
+  <<GET1_TGT: Memory.get loc to mem1_tgt = None>> /\
+  <<GET2_TGT: Memory.get loc to mem2_tgt = Some (from, msg)>>.
+Proof.
+  exploit Memory.cap_inv; try exact CAP_SRC; eauto. i. des; try congr.
+  - subst.
+    exploit sim_memory_adjacent_src; try exact x1; eauto. i. des.
+    inv CAP_TGT. exploit MIDDLE; eauto. i. splits; auto.
+    inv x3. apply EMPTY; eauto. refl.
+  - subst.
+    erewrite sim_memory_max_ts; eauto.
+    inv CAP_TGT. splits; auto.
+    { destruct (Memory.get loc (Time.incr (Memory.max_ts loc mem1_tgt)) mem1_tgt) as [[]|] eqn:MAX; ss.
+      exploit Memory.max_ts_spec; eauto. i. des.
+      specialize (Time.incr_spec (Memory.max_ts loc mem1_tgt)). i. timetac.
+    }
+    { hexploit Memory.max_ts_spec.
+      { eapply MEM1_TGT. }
+      i. des. eapply BACK; eauto.
+    }
+Qed.
+
+Lemma sim_memory_cap_get_tgt
+      mem1_src mem2_src
+      mem1_tgt mem2_tgt
+      loc from to msg
+      (MEM1: sim_memory mem1_src mem1_tgt)
+      (CAP_SRC: Memory.cap mem1_src mem2_src)
+      (CAP_TGT: Memory.cap mem1_tgt mem2_tgt)
+      (MEM1_SRC: Memory.closed mem1_src)
+      (MEM1_TGT: Memory.closed mem1_tgt)
+      (GET1_TGT: Memory.get loc to mem1_tgt = None)
+      (GET2_TGT: Memory.get loc to mem2_tgt = Some (from, msg)):
+  <<MSG: msg = Message.reserve>> /\
+  <<GET1_SRC: Memory.get loc to mem1_src = None>> /\
+  <<GET2_SRC: Memory.get loc to mem2_src = Some (from, msg)>>.
+Proof.
+  exploit Memory.cap_inv; try exact CAP_TGT; eauto. i. des; try congr.
+  - subst.
+    exploit sim_memory_adjacent_tgt; try exact x1; eauto. i. des.
+    inv CAP_SRC. exploit MIDDLE; eauto. i. splits; auto.
+    inv x3. apply EMPTY; eauto. refl.
+  - subst.
+    erewrite <- sim_memory_max_ts; eauto.
+    inv CAP_SRC. splits; auto.
+    { destruct (Memory.get loc (Time.incr (Memory.max_ts loc mem1_src)) mem1_src) as [[]|] eqn:MAX; ss.
+      exploit Memory.max_ts_spec; eauto. i. des.
+      specialize (Time.incr_spec (Memory.max_ts loc mem1_src)). i. timetac.
+    }
+    { hexploit Memory.max_ts_spec.
+      { eapply MEM1_SRC. }
+      i. des. eapply BACK; eauto.
+    }
+Qed.
+
+Lemma sim_memory_cap
+      mem1_src mem2_src
+      mem1_tgt mem2_tgt
+      (MEM1: sim_memory mem1_src mem1_tgt)
+      (CAP_SRC: Memory.cap mem1_src mem2_src)
+      (CAP_TGT: Memory.cap mem1_tgt mem2_tgt)
+      (MEM1_SRC: Memory.closed mem1_src)
+      (MEM1_TGT: Memory.closed mem1_tgt):
+  <<MEM2: sim_memory mem2_src mem2_tgt>>.
+Proof.
+  econs; i; try split; i.
+  - inv H.
+    destruct (Memory.get loc to mem1_src) as [[]|] eqn:GET1.
+    + inv CAP_SRC. exploit SOUND; eauto. intros x.
+      rewrite x in GET. inv GET.
+      eapply cap_covered; eauto.
+      inv MEM1. eapply Interval.le_mem; eauto. econs; ss.
+      { eapply Time.bot_spec. }
+      { erewrite <- sim_memory_max_ts; eauto.
+        eapply Memory.max_ts_spec in GET1. des.
+        etrans; eauto. left. eapply Time.incr_spec.
+      }
+    + exploit sim_memory_cap_get_src; eauto. i. des.
+      econs; eauto.
+  - inv H.
+    destruct (Memory.get loc to mem1_tgt) as [[]|] eqn:GET1.
+    + inv CAP_TGT. exploit SOUND; eauto. intros x.
+      rewrite x in GET. inv GET.
+      eapply cap_covered; try apply CAP_SRC; eauto.
+      inv MEM1. eapply Interval.le_mem; eauto. econs; ss.
+      { eapply Time.bot_spec. }
+      { erewrite sim_memory_max_ts; eauto.
+        eapply Memory.max_ts_spec in GET1. des.
+        etrans; eauto. left. eapply Time.incr_spec.
+      }
+    + exploit sim_memory_cap_get_tgt; eauto. i. des.
+      econs; eauto.
+  - destruct (Memory.get loc to mem1_tgt) as [[]|] eqn:GET1.
+    + inv CAP_TGT. exploit SOUND; eauto. intros x.
+      rewrite x in GET. inv GET.
+      inv MEM1. exploit MSG; eauto. i. des.
+      inv CAP_SRC. exploit SOUND; eauto. i.
+      esplits; eauto.
+    + exploit sim_memory_cap_get_tgt; eauto. i. des.
+      esplits; eauto. refl.
+  - destruct (Memory.get loc to mem1_src) as [[]|] eqn:GET1.
+    + inv CAP_SRC. exploit SOUND; eauto. intros x.
+      rewrite x in H. inv H.
+      inv MEM1. rewrite RSV in GET1.
+      inv CAP_TGT. exploit SOUND0; eauto.
+    + exploit sim_memory_cap_get_src; eauto. i. des. auto.
+  - destruct (Memory.get loc to mem1_tgt) as [[]|] eqn:GET1.
+    + inv CAP_TGT. exploit SOUND; eauto. intros x.
+      rewrite x in H. inv H.
+      inv MEM1. rewrite <- RSV in GET1.
+      inv CAP_SRC. exploit SOUND0; eauto.
+    + exploit sim_memory_cap_get_tgt; eauto. i. des. auto.
+Qed.
+
 Lemma sim_memory_closed_timemap
       mem_src mem_tgt
       tm
